Lean4Lean/Experimental/UniqueTyping.lean
@@ -112,9 +112,10 @@ theorem HasTypeS.uniq {Γ : List SExpr} {e A B : SExpr} {b₁ b₂ : Bool}
     let .app h_f' _ := H2_s
     obtain ⟨_, h_pi_eq⟩ := ih_f hΓ h_f'
     obtain ⟨_, _, h_A_eq, h_B_eq⟩ := SExpr.forallE_inv hΓ h_pi_eq
+    have hΓA : Ctx.WF (A :: Γ') := ⟨hΓ, _, h_A_eq.hasType.1⟩
     have W : Ctx.SubstEq Γ' (.one a) (.one a) (A :: Γ') :=
       .cons .nil h_A_eq.hasType.1 (by simpa using h_a.hasType)
-    exact transport (h_B_eq.subst W)
+    exact transport (h_B_eq.subst hΓA W)
   | @lam _ _ _ _ body h_A _ _ ih_body =>
     obtain ⟨_, H2_s, transport⟩ := H2.toStructural
     let .lam _ h_body' := H2_s
